Extending test case for #21

examples/unit-tests/bug21.fst
@@ -3,9 +3,30 @@ module Bug21
 val constfun : 'a -> 'b -> Tot 'a
 let constfun x _ = x
 
-
 val ftrue_int : int -> Tot bool
 let ftrue_int = constfun true
 
 val ftrue : 'b -> Tot bool
 let ftrue = constfun true
+
+val my_override : ('a -> Tot 'b) -> 'a -> 'b -> Tot ('a -> Tot 'b)
+let my_override f k x k' = if k = k' then x else f k'
+
+val fmostlytrue : int -> Tot bool
+let fmostlytrue x = my_override (my_override ftrue 1 false) 3 false x
+
+val override_example1 : unit -> Fact unit
+      (ensures (fmostlytrue 0 = true))
+let override_example1 () = ()
+
+val override_example2 : unit -> Fact unit
+      (ensures (fmostlytrue 1 = false))
+let override_example2 () = ()
+
+val override_example3 : unit -> Fact unit
+      (ensures (fmostlytrue 2 = true))
+let override_example3 () = ()
+
+val override_example4 : unit -> Fact unit
+      (ensures (fmostlytrue 3 = false))
+let override_example4 () = ()
